

Diffrentiation = अवकलन

07. Quotient rule

$$\frac{d}{dx} \left(\frac{u}{v} \right) = \frac{v \frac{d}{dx} u - u \frac{d}{dx} v}{v^2}$$

$$y = \frac{x^2 - 1}{x^2 + 1}$$

$$\frac{d}{dx} \left(\frac{x^2 - 1}{x^2 + 1} \right) = \frac{(x^2 + 1) \frac{d}{dx} (x^2 - 1) - (x^2 - 1) \frac{d}{dx} (x^2 + 1)}{(x^2 + 1)^2}$$

$$= \frac{(x^2 + 1) \left[\frac{d}{dx} (x^2) - \frac{d}{dx} (1) \right] - (x^2 - 1) \left[\frac{d}{dx} (x^2) + \frac{d}{dx} (1) \right]}{(x^2 + 1)^2}$$

$$= \frac{(x^2 + 1)[2x^{2-1} - 0] - (x^2 - 1)[2x^{2-1} + 0]}{(x^2 + 1)^2}$$

$$= \frac{(x^2 + 1)[2x - 0] - (x^2 - 1)[2x + 0]}{(x^2 + 1)^2}$$

$$\frac{(x^2 + 1)[2x] - (x^2 - 1)[2x]}{(x^2 + 1)^2}$$

$$\frac{4x}{(x^2 + 1)^2} \text{ Ans}$$

$$y = \frac{2x}{4x+3}$$

$$\frac{d}{dx} \left(\frac{2x}{4x+3} \right) = \frac{(4x+3) \frac{d}{dx}(2x) - (2x) \frac{d}{dx}(4x+3)}{(4x+3)^2}$$

$$= \frac{(4x+3) 2 \frac{d}{dx}(x) - (2x) \left[\frac{d}{dx}(4x) + \frac{d}{dx}(3) \right]}{(4x+3)^2}$$

$$= \frac{2(4x+3) - 2x[4(1) + (0)]}{(4x+3)^2}$$

$$= \frac{8x+6-8x}{(4x+3)^2} = \frac{6}{(4x+3)^2} \text{ Ans}$$

$$y = \frac{2x-3}{2x+1}$$

$$\frac{d}{dx} \left(\frac{2x-3}{2x+1} \right) = \frac{(2x+1) \frac{d}{dx}(2x-3) - (2x-3) \frac{d}{dx}(2x+1)}{(2x+1)^2}$$

$$= \frac{(2x+1) \left[\frac{d}{dx}(2x) - \frac{d}{dx}(3) \right] - (2x-3) \left[\frac{d}{dx}(2x) + \frac{d}{dx}(1) \right]}{(2x+1)^2}$$

$$= \frac{(2x+1) \left[2 \frac{d}{dx}(x) - \frac{d}{dx}(3) \right] - (2x-3) \left[2 \frac{d}{dx}(x) + \frac{d}{dx}(1) \right]}{(2x+1)^2}$$

$$= \frac{(2x+1)[2(1) - (0)] - (2x-3)[2(1) + (0)]}{(2x+1)^2}$$

$$= \frac{(2x+1)[2] - (2x-3)[2]}{(2x+1)^2}$$

$$= \frac{(1)[2] - (-3)[2] = 2+6}{(2x+1)^2} = \frac{8}{(2x+1)^2} \text{ Ans.}$$